src/Proofs.v
@@ -8,34 +8,64 @@ Notation "[ ]" := nil.
 Notation "[ x ; .. ; y ]" := (cons x .. (cons y nil) ..).
 
 
-Inductive simList {X:Type} : list X -> list X -> Prop :=
-  | simL_eq l1 l2 : eq l1 l2 -> simList l1 l2
-  | simL_consS h1 t1 h2 t2 : eq h1 h2 -> simList t1 t2 -> simList (h1::t1) (h2::t2)
-  | simL_cons1 h1 t1 h2 t2 : eq_nat (length t1) (length t2 + 1)
-                         -> simList t1 (h2::t2)
-                         -> simList (h1::t1) (h2::t2)
-  | simL_cons2 h1 t1 h2 t2 : eq_nat (length t1 + 1) (length t2)
-                         -> simList (h1::t1) t2
-                         -> simList (h1::t1) (h2::t2)
-.
+Inductive simList {X:Type} : nat -> list X -> list X -> Prop :=
+  | simL_eq l1 l2 : forall n, eq l1 l2 -> simList n l1 l2
+  | simL_cons h t1 t2 : forall n, simList n t1 t2 -> simList n (cons h t1) (cons h t2)
+  | simL_cons1 h1 l1 l2 : forall n, simList n l1 l2
+                         -> simList (S n) (cons h1 l1) l2
+  | simL_cons2 l1 h2 l2 : forall n, simList n l1 l2
+                         -> simList (S n) l1 (cons h2 l2)
+  | simL_weak l1 l2 : forall d, simList d l1 l2 -> simList (S d) l1 l2.
 
-Example simEx1 : simList [1;2] [2].
-Proof. apply simL_cons1. reflexivity. apply simL_eq. reflexivity. Qed.
+Example simEx1 : simList 1 [1;2] [2].
+Proof. apply simL_cons1. apply simL_eq. reflexivity. Qed.
 
-Example simEx2 : simList [1;2;3;4] [1;3;4].
-Proof. apply simL_consS. reflexivity.
-  apply simL_cons1. reflexivity. apply simL_eq. reflexivity. Qed.
+Example simEx2 : simList 1 [1;2;3;4] [1;3;4].
+Proof. apply simL_cons. 
+  apply simL_cons1. apply simL_eq. reflexivity. Qed.
 
+Example simEx3 : simList 1 [] [1].
+Proof. apply simL_cons2. apply simL_eq. reflexivity. Qed.
+
+Lemma listConsEq : forall (X:Type) (a:X) l1 l2,
+  l1 = l2 -> a::l1 = a::l2.
+Proof. intros. rewrite H. reflexivity. Qed.
+
+Lemma listConsEq' : forall (X:Type) (a:X) l1 l2,
+  a::l1 = a::l2 -> l1 = l2.
+Proof. intros. inversion H. reflexivity. Qed.
+
+Lemma simLZeroEq : forall (X:Type) (l1 l2:list X),
+  simList 0 l1 l2 -> l1 = l2.
+Proof. intros X l1. induction l1. intros.
+  inversion H. apply H0.
+  intros. induction l2. inversion H. inversion H0.
+  inversion H. apply H0.
+  apply listConsEq. apply IHl1. apply H2.
+Qed.
+
+(*
+Lemma simLOneOff : forall (X:Type) (x1 x2:X) (l1 l2:list X),
+  simL 1 (x1::l1) (x2::l2) -> x1<>x2 -> l1 = l2.
+*)
 
 Inductive all {X : Type} (P : X -> Prop) : list X -> Prop :=
   | all_nil : all P []
   | all_cons x l : P x -> all P l -> all P (x :: l).
 
-Inductive simNat : nat -> nat -> Prop :=
-  | simN_eq n1 n2 : eq_nat n1 n2 -> simNat n1 n2
-  | simN_l n1 n2 : eq_nat (S n1) n2 -> simNat n1 n2
-  | simN_r n1 n2 : eq_nat n1 (S n2) -> simNat n1 n2
-.
+Inductive simNat : nat -> nat -> nat -> Prop :=
+  | simN_eq n1 n2 : forall d, eq_nat n1 n2 -> simNat d n1 n2
+  | simN_S n1 n2 : forall d, simNat d n1 n2 -> simNat d (S n1) (S n2)
+  | simN_l n1 n2 : forall d, simNat d n1 n2 -> simNat (S d) (S n1) n2
+  | simN_r n1 n2 : forall d, simNat d n1 n2 -> simNat (S d) n1 (S n2)
+  | simN_weak n1 n2 : forall d, simNat d n1 n2 -> simNat (S d) n1 n2.
+
+Lemma simNatPlus : forall (d n s1 s2 : nat),
+  simNat d s1 s2 -> simNat d (n+s1) (n+s2).
+Proof. intros. induction n.
+  simpl. apply H.
+  simpl. apply simN_S. apply IHn.
+Qed.
 
 Fixpoint sumList (l : list nat) : nat :=
   match l with
@@ -47,14 +77,26 @@ Example sumListEx1 : eq_nat 10 (sumList [1;2;3;4]).
 Proof. reflexivity. Qed.
 
 
-Lemma foo : forall (Arg Arg' : list nat),
-  simList Arg Arg' ->
+
+Lemma foo : forall (Arg Arg' : list nat) (d:nat),
+  simList d Arg Arg' ->
   all (fun x => x <= 1) Arg ->
   all (fun x => x <= 1) Arg' ->
-  simNat (sumList Arg) (sumList Arg').
-Proof. intros. inversion H.
-  rewrite H2. apply simN_eq. apply eq_nat_refl.
-  rewrite H2. simpl.
+  simNat d (sumList Arg) (sumList Arg').
+Proof. intros. induction H.
+  rewrite H. apply simN_eq. apply eq_nat_refl.
+  simpl. apply simNatPlus. apply IHsimList.
+    inversion H0. apply H5. inversion H1. apply H5.
+  inversion H0. inversion H4. simpl. apply simN_l. apply IHsimList.
+    apply H5. apply H1.
+    inversion H7. simpl. apply simN_weak. apply IHsimList.
+      apply H5. apply H1.
+  inversion H1. inversion H4. simpl. apply simN_r. apply IHsimList.
+    apply H0. apply H5.
+    inversion H7. simpl. apply simN_weak. apply IHsimList.
+      apply H0. apply H5.
+  apply simN_weak. apply IHsimList. apply H0. apply H1.
+Qed.
 
 
 
